@prefix dc: <http://purl.org/dc/elements/1.1/> .
@prefix dcterms: <http://purl.org/dc/terms/> .
@prefix rdf: <http://www.w3.org/1999/02/22-rdf-syntax-ns#> .
@prefix rdfs: <http://www.w3.org/2000/01/rdf-schema#> .
@prefix skos: <http://www.w3.org/2004/02/skos/core#> .
@prefix skosxl: <http://www.w3.org/2008/05/skos-xl#> .
@prefix xml: <http://www.w3.org/XML/1998/namespace> .
@prefix xsd: <http://www.w3.org/2001/XMLSchema#> .
@prefix profLevel: <http://purl.org/dcx/ld4pe-vocabs/proficiencyLevel/>.

profLevel: a skos:ConceptScheme ;
    dc:title "Educational Audience Proficiant Levels"@en-us ;
    dc:description """This vocabulary defines the proficiency level or levels of the 
        intended learners for whom a learning resource is intended or useful."""@en-us ;    
    dc:creator "DCMI/LD4PE Task Group"@en-us ;
    dcterms:created "2015-09-22"^^dcterms:W3CDTF ;
    dcterms:source """Based on the Office of Human Resources, U.S. National Institutes of Health
        proficiency scale levels for competencies: 
        https://hr.od.nih.gov/workingatnih/competencies/proficiencyscale.htm"""@en-us .

profLevel:fundamentalAwareness a skos:Concept ;
    skos:prefLabel "fundamental awareness"@en-us ;
    skosxl:preflabel profLevel:label-fundamentalAwareness ;
    skos:definition """Basic level: Persons in this class are beginning development of a 
        knowledge and understanding of the common, basic techniques, and concepts. Focus 
        is on learning."""@en-us ;
    skos:inScheme profLevel: .
    
profLevel:novice a skos:Concept ;
    skos:prefLabel "novice"@en-us ;
    skosxl:preflabel profLevel:label-novice ;    
    skos:definition """Limited experience: Persons in this class have the proficiency 
        gained in a classroom and/or experimental scenarios or as a trainee 
        on-the-job. Focus is on developing through experiment in application."""@en-us ;
    skos:scopeNote """Persons at this level of proficiency are expected to need help when 
        performing the competency or set of competencies. Persons at this level are capable 
        of understanding and can discuss terminology, concepts, principles, and issues related 
        to this competency or set of competencies."""@en-us ;
    skos:inScheme profLevel: .  

profLevel:intermediate a skos:Concept ;
    skos:prefLabel "intermediate"@en-us ;
    skosxl:preflabel profLevel:label-intermediate ;    
    skos:definition """Semi-independent practical application: Proficient persons in this class 
        are able to successfully complete the tasks required by the competency or set of 
        competencies."""@en-us ;
    skos:scopeNote """Help from an expert may be required from time to time, but the person can 
        usually perform the skill(s) independently. Focus is on applying and enhancing knowledge 
        or skill.  Person may have applied this competency to situations occasionally while 
        needing minimal guidance to perform successfully."""@en-us ;
    skos:inScheme profLevel: .  
    
profLevel:advanced a skos:Concept ;
    skos:prefLabel "advanced"@en-us ;
    skosxl:preflabel profLevel:label-advanced ;    
    skos:definition """Applied theory: Persons in this class can perform the actions associated 
        with this skill or skill set without assistance. Focus is on broad organizational/professional 
        issues."""@en-us ;
    skos:scopeNote """Person is recognized within his or her immediate organization as \"a person to 
        ask\" when difficult questions arise regarding the skill or skills embodied. Person is capable 
        of coaching others in the application of this competency by translating complex nuances 
        relating to this competency into easy to understand terms."""@us-en;
    skos:inScheme profLevel: .
    
profLevel:expert a skos:Concept ;
    skos:prefLabel "expert"@en-us ;
    skosxl:preflabel profLevel:label-expert ;    
    skos:definition """Recognized Authority: Persons can provide guidance, troubleshoot and answer 
        questions related to this area of expertise and the field where the skill or skill set is 
        used. Focus is strategic."""@us-en ;
    skos:scopeNote """Persons have created new applications for and/or lead the development of 
        reference and resource materials for this competency. Persons are able to diagram or 
        explain the relevant process elements and issues in relation to organizational trends 
        in sufficient detail during discussions and presentations, to foster a greater understanding 
        among internal and external colleagues and constituents."""@en-us ;
    skos:inScheme profLevel: .
    
#============================= 
# EXTENDED LABELS
#=============================     
    
profLevel:label-fundamentalAwareness a skosxl:label ;
    skosxl:literalForm "fundamental awareness"@en-US . 
    
profLevel:label-novice a skosxl:label ;
    skosxl:literalForm "novice"@en-US .
    
profLevel:label-intermediate a skosxl:label ;
    skosxl:literalForm "intermediate"@en-US . 
    
profLevel:label-advanced a skosxl:label ;
    skosxl:literalForm "advanced"@en-US .
    
profLevel:label-expert a skosxl:label ;
    skosxl:literalForm "expert"@en-US .                  
